

Elin

$$\begin{aligned}
 \textcircled{1} \quad F(x, y, z) &= xy + x'z + yz + (x \cdot x') \\
 &= z(x' + y) + xy + (x \cdot x') \\
 &= z(x' + y) + x(x' + y) \\
 &\Rightarrow (x + z) \cdot (x' + y)
 \end{aligned}$$

$$\begin{aligned}
 \textcircled{2} \quad (x + y)(x' + z)(y + z) &= (x + y)(x' + z) \\
 &= (x + y)(x' + z)(y + z + x \cdot x') \\
 &= (x + y)(x' + z)(x + y + z)(x' + y + z) \\
 &= (x + y)(\underbrace{1 + z})_1 (x' + z)(\underbrace{1 + y})_1 \\
 &\Rightarrow (x + y)(x' + z)
 \end{aligned}$$

a)

A	B	C	D	B'D	A'D	BD	F	
0	0	0	0	0	0	0	0	m ₀
0	0	0	1	1	1	0	1	→ a'b'c'd
0	0	1	0	0	0	0	0	m ₂
0	0	1	1	1	1	0	1	→ a'b'cd
0	1	0	0	0	0	0	0	m ₄
0	1	0	1	0	1	1	1	→ a'bc'd
0	1	1	0	0	0	0	0	m ₆
0	1	1	1	0	1	1	1	→ a'bcd
1	0	0	0	0	0	0	0	m ₈
1	0	0	1	1	0	0	1	→ ab'c'd
1	0	1	0	0	0	0	0	m ₁₀
1	0	1	1	1	0	0	1	→ ab'cd
1	1	0	0	0	0	0	0	m ₁₂
1	1	0	1	0	0	1	1	→ abc'd
1	1	1	0	0	0	0	0	m ₁₄
1	1	1	1	0	0	1	1	→ abcd
								m ₁₅

Sum of minterms $\Sigma(1, 3, 5, 7, 9, 11, 13, 15)$ Product of maxterm $\Pi(0, 2, 4, 6, 8, 10, 12, 14)$

$$F(A, B, C, D) = B'D + A'D + BD$$

$$\begin{aligned}
 D(B' + A' + B) &= D(\underbrace{1 + A'})_1 = D
 \end{aligned}$$

$$\begin{aligned}
 A + A' &= 1 \\
 A' + 1 &= 1
 \end{aligned}$$

b)